$$\begin{array}{|c|c|c|}
\hline

\bint x^a dx = \cfrac{x^{a + 1}}{a + 1} + c, a \ne -1 &
\bint \cfrac{dx}{x} = \ln |x| + c &
\bint e^x dx = e^x + c
\\\hline

\bint \sin x dx = -\cos x + c &
\bint \cos x dx = \sin x + c &
\bint \cfrac{dx}{\cos^2 x} = \tg x + c
\\\hline

\bint \cfrac{dx}{\sin^2 x} = -\ctg x + c &
\bint \cfrac{dx}{1 + x^2} = \arctg x + c &
\bint \cfrac{dx}{\sqrt{1 - x^2}} = \arcsin x + c
\\\hline

\bint \cfrac{dx}{\sqrt{1 + x^2}} = \ln (x + \sqrt{1 + x^2}) + c
\\\hline
\end{array}$$